proofs/Verify_seq_to_array_old.v
@@ -9,44 +9,184 @@ Implicit Types p q : loc.
 
 From Proofs Require Import Seq_to_array_old.
 
+(** Lazy values: a lazy value of type [a] is represented at type [unit->'a].
+    [Lazyval P f] asserts that [f] is a lazy value whose evaluation produces
+    a value satisfying the (pure) predicate [P]. *)
 
+Definition Lazyval A `{EA:Enc A} (P:A->Prop) (f:val) : Prop :=
+  SPEC_PURE (f tt) POST (fun a => \[P a]). 
 
-Fixpoint MSeq A `{EA: Enc A} (ls: list A) (f: val) : hprop :=
-  match ls with
-  | nil => \[ SPEC (f val_unit) PRE \[]  POST \[= (Nil: node_ A) ] ]
-  | h :: t =>
-      \exists nxt,
-          \[ SPEC (f val_unit) PRE \[] POST \[= Cons h nxt]] \*
-           @MSeq A EA t nxt
-  end.
+Definition LSeq_node A `{EA:Enc A} (LSeq: list A -> t_ A -> Prop) (L:list A) (s: node_ A) : Prop :=
+ match L with
+ | nil => s = Nil
+ | x::L' => exists f', s = Cons x f' /\ LSeq L' f'
+ end. 
 
-Fixpoint itoa (m: nat) (n: nat) :=
+Lemma LSeq_node_Nil : forall A (EA:Enc A) (LSeq: list A -> t_ A -> Prop),
+  LSeq_node LSeq (@nil A) Nil.
+Proof using. intros. simpl. auto. Qed.
+
+Lemma LSeq_node_Cons : forall A (EA: Enc A) (LSeq: list A -> t_ A-> Prop) (x: A) (L': list A) (f: func),
+  LSeq L' f ->
+  LSeq_node LSeq (x::L') (Cons x f).
+Proof using. introv Hf. simpl. exists* f. Qed.
+
+Fixpoint LSeq A `{EA: Enc A} (L: list A) (f: t_ A) : Prop :=
+  Lazyval (LSeq_node (@LSeq A EA) L) f.
+
+Lemma LSeq_intro : forall A `{EA:Enc A} (L:list A) (f: t_ A),
+  SPEC_PURE (f tt) POST (fun a => \[(LSeq_node (@LSeq A EA) L) a]) ->
+  LSeq L f.
+Proof using.
+  (* Coq forces us to do a case analysis on L in order to unfold the fixpoint definition. *)
+  intros. unfold LSeq, Lazyval. destruct L; simpl; xapplys* H.
+Qed.
+
+Lemma LSeq_if : forall A `{EA:Enc A} (L:list A) (f: t_ A),
+    LSeq L f ->
+    (SPEC_PURE (f tt) POST (fun a => \[(LSeq_node (@LSeq A EA) L) a])) .
+Proof using.
+  intros A EA L; case L as [| hd tl]; intros f; simpl; auto.
+Qed.
+
+Fixpoint itoa (m: int) (n: nat) :=
   match n with
   | O => nil
-  | S n => Z.of_nat m :: itoa (S m) n
+  | S n => m :: itoa (m + 1) n
   end.
 
-Lemma int_range_spec : forall m n,
-   0 <= m -> 0 <= n  ->
-  SPEC (int_range m n)
-    PRE \[]
-    POST (fun f => MSeq (itoa (Z.to_nat m) (Z.to_nat n)) f).
+Lemma itoa_pos : forall start nb,
+  nb > 0 ->
+  itoa start (Z.to_nat nb) = start :: itoa (start+1) (Z.to_nat (nb-1)).
 Proof using.
-  intros m n Hm Hn; gen Hm Hn.
-  induction_wf IH: (downto 0) n.
-  intros Hm Hn.
-  xcf.
+  introv Hnb.
+  case_eq (to_nat nb); try (intros H; math).
+  intros n' Hnb'; simpl; apply f_equal.
+  assert (n' = to_nat (nb - 1)) as H. {math.}
+  rewrite H; auto.
+Qed.
+
+Lemma int_range_lspec : forall start nb,
+   0 <= nb  ->
+  SPEC_PURE (int_range start nb)
+    POST (fun f => \[ LSeq (itoa start (Z.to_nat nb)) f ]).
+Proof using.
+  introv. gen start. induction_wf IH: (downto 0) nb; intros. xcf.
+  xlet. xvals. apply LSeq_intro. xapp. clear Spec_f0__. xif;=> C.
+  { xapp; try (hnf; math). intros s' HS'. xvals. rewrite itoa_pos; try math.
+    applys_eq* LSeq_node_Cons. }
+  { xvals. applys_eq LSeq_node_Nil. math_rewrite (nb = 0). auto. }
+Qed.  
+
+Lemma fold_spec : forall A `{Enc A} B `{Enc B} (ls: list A) f (init : B) s (fp: B -> A -> B),
+    (forall acc v,
+        SPEC_PURE (f acc v)
+        POST \[= fp acc v]) ->
+  SPEC (fold f init s)
+    PRE \[LSeq ls s]
+    POST \[= List.fold_left fp ls init].
+Proof using.
+  introv Hspec. gen s init. induction ls; xcf.
+  { xpull ;=> HLseq. apply LSeq_if in HLseq. xapp. xmatch. xvals. auto. }
+  { xpull ;=> HLseq. apply LSeq_if in HLseq. xapp ;=> nxt'. simpl LSeq_node;=>[nxt [-> Hnxt]].
+    xmatch. xapp. xapp; auto. xsimpl. auto. }
+Qed.
+
+Lemma length_spec : forall A `{Enc A} (ls: list A) s,
+  SPEC (length'__ s)
+    PRE \[LSeq ls s]
+    POST (fun len => \[ len = length ls ]).
+Proof using.
+  xcf; auto. xlet (fun f => forall (acc: int) (v: A), SPEC_PURE (f acc v) POST \[= (acc + 1) ]).
+  { xval. xsimpl. math. }
+  xpull ;=> Hs.
+  xapp (@fold_spec _ _ _ _ ls f0__ 0 s (fun (acc: int) _ => acc + 1)); auto.
+  xsimpl.
+  clear.
+  cut (forall a, List.fold_left (fun (acc : credits) (_ : A) => acc + 1) ls a = a + length ls). {
+    intros H.
+    apply H.
+  }
+  induction ls.
+  - intros a; simpl; rewrite length_nil; auto; math.
+  - intros a'; simpl. rewrite IHls. rewrite length_cons; math.
+Qed.
+
+Lemma iteri_spec : forall A `{EA: Enc A} (l: list A) (f: func) (s: t_ A),
+  forall (I: list A -> hprop),
+  (forall x t r i, (l = t++x::r) -> i = length (t) ->
+     SPEC (f i x) PRE (I t) POSTUNIT (I (t&x))) ->  
+  SPEC (iteri f s)
+    PRE (\[@LSeq A EA l s] \* I nil)
+    POSTUNIT (I l).
+Proof using.
+  =>> M. xcf; auto.
   xlet.
-  xval.
-  case_eq (Z.to_nat n). 
-  - intros Heq. simpl MSeq.
-    xsimpl.
-    applys~ Spec_f0__.
-    Unshelve. exact tt.
-    xif; intro Hcond; try math.
-    xval.
-    xsimpl.
-    auto.
-  - intros n' Hn'; simpl MSeq.
-Admitted.    
-  
+  asserts aux_spec: (
+   forall i r t s,
+     l = t ++ r ->
+     i = length t ->
+     SPEC (aux f s i)
+     PRE (I t \* \[LSeq r s])
+     POSTUNIT (I l)
+                    ).
+  {
+    intro i; induction_wf IH: (upto (length l)) i.
+    intros r t s' Hl Hi.
+    eapply Spec_aux; clear Spec_aux.
+    xpull ;=> HLseq. apply LSeq_if in HLseq.
+    case_eq r.
+    * intros ->. xapp. xmatch. xvals. rewrite app_nil_r in Hl; rewrite Hl; xsimpl.
+    * intros x xs ->. xapp;=>result [nxt_r [-> Hnxt_r]].
+      xmatch. xseq. xapp~ (M x t xs).
+      xapp.
+      ** unfold upto. split; try math.
+         rewrite Hl; rewrite length_app; rewrite Hi; rewrite length_cons.
+         math.
+      ** rewrite Hl. rewrite <- app_cons_r. auto.
+      ** rewrite length_last. math.
+      ** auto.
+      ** xsimpl.
+  }
+  xpull;=> Hlseq.
+  xapp (aux_spec 0 l); auto; try xsimpl.
+Qed.
+
+Hint Extern 1 (RegisterSpec iteri) => Provide iteri_spec.
+
+Lemma to_array_spec : forall A `{EA:Enc A} (l:list A) (s:func),
+  SPEC (to_array s)
+    PRE (\[LSeq l s])
+    POST (fun a => a ~> Array l).
+Proof using.
+  xcf.
+  xpull ;=> HLseq; apply LSeq_if in HLseq.
+  case_eq l.
+  - intros ->; xapp; xmatch. xapp;=> x; xsimpl.
+  - intros x xs Hl; rewrite Hl in *; xapp ;=> result [nxt_r [-> Hnxt_r]].
+    xmatch.
+    xapp length_spec. {apply LSeq_intro; auto. applys HLseq.}
+    xapp. {math.} => arr data Hdata.
+    xlet.
+    xseq.
+    xapp (@iteri_spec A EA l f0__ s (fun ls => arr ~> Array (ls ++ (make (length l - length ls) x)) )).
+    * {
+      intros y t ys i IHl IHi.
+      xapp Spec_f0__; clear Spec_f0__.
+      xapp.
+      rewrite IHl; rewrite IHi.
+      apply int_index_prove; try math.
+      rewrite <- length_eq. rewrite !length_app. rewrite length_cons. rewrite length_make; try math.
+      xsimpl.
+      rewrite length_last. math_rewrite ((length l - (1 + length t)) = ((length l - length t) - 1)).
+      rewrite (@update_app_r _  _ 0 _ _ _ y IHi); try math.
+      rewrite app_last_l.
+      apply f_equal.
+      rewrite make_eq_cons_make_pred; try (rewrite IHl; rewrite length_app; rewrite length_cons; math).
+      rewrite update_zero.
+      auto.
+    }
+    * apply LSeq_intro; rewrite Hl; eapply HLseq.
+    * rew_list; math_rewrite ((length l - 0) = length l); rewrite Hl; auto.
+    * xvals. math_rewrite ((length l - length l) = 0); rewrite make_zero; rew_list; auto.
+Qed.      
